theories/Testing_Pre_orders/Must/Alternative_Preorder/Acceptance_Set/Equivalence/EquivalenceAS.v
@@ -2,6 +2,7 @@
    Copyright (c) 2024 Nomadic Labs
    Copyright (c) 2024 Paul Laforgue <paul.laforgue@nomadic-labs.com>
    Copyright (c) 2024 Léo Stefanesco <leo.stefanesco@mpi-sws.org>
+   Copyright (c) 2025 Gaëtan Lopez <glopez@irif.fr>
 
    Permission is hereby granted, free of charge, to any person obtaining a copy
    of this software and associated documentation files (the "Software"), to deal
@@ -22,52 +23,30 @@
    SOFTWARE.
 *)
 
-Require ssreflect.
-Require Import Coq.Unicode.Utf8.
-Require Import Coq.Lists.List.
-Import ListNotations.
-Require Import Coq.Program.Equality.
-Require Import Coq.Wellfounded.Inverse_Image.
-Require Import Coq.Logic.JMeq.
-Require Import Coq.Program.Wf Setoid.
-Require Import Coq.Program.Equality.
-From Coq.Logic Require Import ProofIrrelevance.
-From stdpp Require Import base countable finite gmap list finite base decidable finite gmap.
-From Must Require Import ActTau InputOutputActions gLts Bisimulation Lts_OBA Lts_OBA_FB Lts_FW FiniteImageLTS
-            Subset_Act Must SoundnessAS CompletenessAS EquivalenceAS StateTransitionSystems
-              GeneralizeLtsOutputs Termination WeakTransitions Convergence  
-               InteractionBetweenLts MultisetLTSConstruction ForwarderConstruction ParallelLTSConstruction
-               Testing_Predicate DefinitionAS DefinitionCI SoundnessCI CompletenessCI.
+From stdpp Require Import base decidable gmap finite.
+From Coq Require Import ssreflect.
+From Coq.Program Require Import Equality.
+From Must Require Import gLts Bisimulation Lts_OBA Lts_FW Lts_OBA_FB StateTransitionSystems Termination
+    Must Bar CompletenessAS SoundnessAS Lift Subset_Act FiniteImageLTS WeakTransitions Convergence
+    InteractionBetweenLts MultisetLTSConstruction ForwarderConstruction ParallelLTSConstruction ActTau
+    Testing_Predicate DefinitionAS MustE.
 
-Theorem eqx `{@FiniteImagegLts A L HL LtsP, @FiniteImagegLts B L HL LtsQ} 
-  `{PreAP : @PreExtAction L HL A FinA PreA PreA_eq PreA_countable 𝝳 Φ LtsP}
-  `{PreAQ : @PreExtAction L HL B FinA PreA PreA_eq PreA_countable 𝝳 Φ LtsQ}
-  (X : gset A) (q : B) :
-  X ≼ₓ q <-> X ⩽ q.
-Proof.
-  split.
-  - eapply copre_if_prex.
-  - intros hco. split. now eapply prex1_if_copre. now eapply prex2_if_copre.
-Qed.
-
-Section eq_contextual.
-
-  Context `{H : ExtAction A}.
+Section preorder.
+  Context `{attaboy : E -> Prop}.
+  Context `{attaboy_dec : forall e, Decision (attaboy e)}.
+  Context `{P : Type}.
+  Context `{Q : Type}.
+  Context `{H : !ExtAction A}.
   Context `{gLtsP : !gLts P A, !FiniteImagegLts P A}.
   Context `{gLtsQ : !gLts Q A, !FiniteImagegLts Q A}.
-  Context `{gLtsE : !gLts E A, !FiniteImagegLts E A}.
+  Context `{gLtsE : !gLts E A, !FiniteImagegLts E A, gLtsEqE: !gLtsEq E A, !Testing_Predicate E A attaboy}.
+  Context `{@Prop_of_Inter P E A parallel_inter H gLtsP gLtsE}.
+  Context `{@Prop_of_Inter Q E A parallel_inter H gLtsQ gLtsE}.
 
   Context `{@gLtsObaFB P A H gLtsP gLtsEqP gLtsObaP}.
   Context `{@gLtsObaFB Q A H gLtsQ gLtsEqQ gLtsObaQ}.
   Context `{@gLtsObaFB E A H gLtsE gLtsEqE gLtsObaE}.
 
-  Context `{attaboy : E -> Prop}.
-  Context `{attaboy_dec : forall e, Decision (attaboy e)}.
-  Context `{!Testing_Predicate E A attaboy}.
-
-  (* ************************************************** *)
-  Context `{@Prop_of_Inter P E A parallel_inter H gLtsP gLtsE}.
-  Context `{@Prop_of_Inter Q E A parallel_inter H gLtsQ gLtsE}.
   Context `{@Prop_of_Inter P (mb A) A fw_inter H gLtsP MbgLts}.
   Context `{@Prop_of_Inter (P * mb A) E A parallel_inter H (inter_lts fw_inter) gLtsE}.
   Context `{@Prop_of_Inter Q (mb A) A fw_inter H gLtsQ MbgLts}.
@@ -80,10 +59,18 @@ Section eq_contextual.
   Context `{igen_conv : @gen_spec_conv E _ _ _ _ attaboy Testing_Predicate0 co_of gen_conv}.
   Context `{igen_acc : @gen_spec_acc PreA _ _ E _ _ _ _ attaboy Testing_Predicate0 co_of gen_acc (fun x => 𝝳 (Φ x))}.
 
-  Theorem eq_ctx (p : P) (q : Q) :
-    @pre_extensional P Q _ _ _ attaboy _ p q <-> {[ p ▷ (∅ : mb A) ]} ⩽ q ▷ (∅ : mb A).
+  (* ************************************************** *)
+
+  (** Equivalence between the extensional definition of the contextual preorder and
+      the alternative, inductive characterisation. *)
+  Theorem equivalence_bhv_acc_ctx (p : P) (q : Q) :
+    @pre_extensional P Q _ _ _ attaboy _ p q <-> (p, ∅) ≼ (q, ∅).
   Proof.
-    rewrite <- eqx, <- alt_set_singleton_iff.
-    now rewrite equivalence_bhv_acc_ctx.
+    split.
+    - intros hpre%pre_extensional_eq.
+      now eapply lift_fw_ctx_pre, completeness_fw in hpre.
+    - intros hpre%soundness_fw.
+      now eapply pre_extensional_eq, lift_fw_ctx_pre.
   Qed.
-End eq_contextual.
+
+End preorder.
