theories/Testing_Pre_orders/Must/Alternative_Preorder/Co_Inductive_Acceptance_Set/Equivalence/EquivalenceCI.v
@@ -1,0 +1,89 @@
+(*
+   Copyright (c) 2024 Nomadic Labs
+   Copyright (c) 2024 Paul Laforgue <paul.laforgue@nomadic-labs.com>
+   Copyright (c) 2024 Léo Stefanesco <leo.stefanesco@mpi-sws.org>
+
+   Permission is hereby granted, free of charge, to any person obtaining a copy
+   of this software and associated documentation files (the "Software"), to deal
+   in the Software without restriction, including without limitation the rights
+   to use, copy, modify, merge, publish, distribute, sublicense, and/or sell
+   copies of the Software, and to permit persons to whom the Software is
+   furnished to do so, subject to the following conditions:
+
+   The above copyright notice and this permission notice shall be included in all
+   copies or substantial portions of the Software.
+
+   THE SOFTWARE IS PROVIDED "AS IS", WITHOUT WARRANTY OF ANY KIND, EXPRESS OR
+   IMPLIED, INCLUDING BUT NOT LIMITED TO THE WARRANTIES OF MERCHANTABILITY,
+   FITNESS FOR A PARTICULAR PURPOSE AND NONINFRINGEMENT. IN NO EVENT SHALL THE
+   AUTHORS OR COPYRIGHT HOLDERS BE LIABLE FOR ANY CLAIM, DAMAGES OR OTHER
+   LIABILITY, WHETHER IN AN ACTION OF CONTRACT, TORT OR OTHERWISE, ARISING FROM,
+   OUT OF OR IN CONNECTION WITH THE SOFTWARE OR THE USE OR OTHER DEALINGS IN THE
+   SOFTWARE.
+*)
+
+Require ssreflect.
+Require Import Coq.Unicode.Utf8.
+Require Import Coq.Lists.List.
+Import ListNotations.
+Require Import Coq.Program.Equality.
+Require Import Coq.Wellfounded.Inverse_Image.
+Require Import Coq.Logic.JMeq.
+Require Import Coq.Program.Wf Setoid.
+Require Import Coq.Program.Equality.
+From Coq.Logic Require Import ProofIrrelevance.
+From stdpp Require Import base countable finite gmap list finite base decidable finite gmap.
+From Must Require Import ActTau InputOutputActions gLts Bisimulation Lts_OBA Lts_OBA_FB Lts_FW FiniteImageLTS
+            Subset_Act Must SoundnessAS CompletenessAS EquivalenceAS StateTransitionSystems
+              GeneralizeLtsOutputs Termination WeakTransitions Convergence  
+               InteractionBetweenLts MultisetLTSConstruction ForwarderConstruction ParallelLTSConstruction
+               Testing_Predicate DefinitionAS DefinitionCI SoundnessCI CompletenessCI MustE.
+
+Theorem eqx `{@FiniteImagegLts A L HL LtsP, @FiniteImagegLts B L HL LtsQ} 
+  `{PreAP : @PreExtAction L HL A FinA PreA PreA_eq PreA_countable 𝝳 Φ LtsP}
+  `{PreAQ : @PreExtAction L HL B FinA PreA PreA_eq PreA_countable 𝝳 Φ LtsQ}
+  (X : gset A) (q : B) :
+  X ≼ₓ q <-> X ⩽ q.
+Proof.
+  split.
+  - eapply copre_if_prex.
+  - intros hco. split. now eapply prex1_if_copre. now eapply prex2_if_copre.
+Qed.
+
+Section eq_contextual.
+
+  Context `{H : ExtAction A}.
+  Context `{gLtsP : !gLts P A, !FiniteImagegLts P A}.
+  Context `{gLtsQ : !gLts Q A, !FiniteImagegLts Q A}.
+  Context `{gLtsE : !gLts E A, !FiniteImagegLts E A}.
+
+  Context `{@gLtsObaFB P A H gLtsP gLtsEqP gLtsObaP}.
+  Context `{@gLtsObaFB Q A H gLtsQ gLtsEqQ gLtsObaQ}.
+  Context `{@gLtsObaFB E A H gLtsE gLtsEqE gLtsObaE}.
+
+  Context `{attaboy : E -> Prop}.
+  Context `{attaboy_dec : forall e, Decision (attaboy e)}.
+  Context `{!Testing_Predicate E A attaboy}.
+
+  (* ************************************************** *)
+  Context `{@Prop_of_Inter P E A parallel_inter H gLtsP gLtsE}.
+  Context `{@Prop_of_Inter Q E A parallel_inter H gLtsQ gLtsE}.
+  Context `{@Prop_of_Inter P (mb A) A fw_inter H gLtsP MbgLts}.
+  Context `{@Prop_of_Inter (P * mb A) E A parallel_inter H (inter_lts fw_inter) gLtsE}.
+  Context `{@Prop_of_Inter Q (mb A) A fw_inter H gLtsQ MbgLts}.
+  Context `{@Prop_of_Inter (Q * mb A) E A parallel_inter H (inter_lts fw_inter) gLtsE}.
+
+  Context `{@PreExtAction A H (P * mb A) FinA PreA PreA_eq PreA_countable 𝝳 Φ (FW_gLts gLtsP)}.
+  Context `{@PreExtAction A H (Q * mb A) FinA PreA PreA_eq PreA_countable 𝝳 Φ (FW_gLts gLtsQ)}.
+  Context `{@AbsAction A H E FinA gLtsE Φ}.
+
+  Context `{igen_conv : @gen_spec_conv E _ _ _ _ attaboy Testing_Predicate0 co_of gen_conv}.
+  Context `{igen_acc : @gen_spec_acc PreA _ _ E _ _ _ _ attaboy Testing_Predicate0 co_of gen_acc (fun x => 𝝳 (Φ x))}.
+
+  Theorem eq_ctx (p : P) (q : Q) :
+    @pre_extensional P Q _ _ _ attaboy _ p q <-> {[ p ▷ (∅ : mb A) ]} ⩽ q ▷ (∅ : mb A).
+  Proof.
+    rewrite <- eqx, <- alt_set_singleton_iff.
+    now rewrite equivalence_bhv_acc_ctx.
+  Qed.
+End eq_contextual.
