theories/Testing_Pre_orders/Must/Alternative_Preorder/Failure_Must/Equivalence/EquivalenceFMS.v
@@ -1,0 +1,136 @@
+(*
+   Copyright (c) 2024 Nomadic Labs
+   Copyright (c) 2024 Paul Laforgue <paul.laforgue@nomadic-labs.com>
+   Copyright (c) 2024 Léo Stefanesco <leo.stefanesco@mpi-sws.org>
+   Copyright (c) 2025 Gaëtan Lopez <glopez@irif.fr>
+
+   Permission is hereby granted, free of charge, to any person obtaining a copy
+   of this software and associated documentation files (the "Software"), to deal
+   in the Software without restriction, including without limitation the rights
+   to use, copy, modify, merge, publish, distribute, sublicense, and/or sell
+   copies of the Software, and to permit persons to whom the Software is
+   furnished to do so, subject to the following conditions:
+
+   The above copyright notice and this permission notice shall be included in all
+   copies or substantial portions of the Software.
+
+   THE SOFTWARE IS PROVIDED "AS IS", WITHOUT WARRANTY OF ANY KIND, EXPRESS OR
+   IMPLIED, INCLUDING BUT NOT LIMITED TO THE WARRANTIES OF MERCHANTABILITY,
+   FITNESS FOR A PARTICULAR PURPOSE AND NONINFRINGEMENT. IN NO EVENT SHALL THE
+   AUTHORS OR COPYRIGHT HOLDERS BE LIABLE FOR ANY CLAIM, DAMAGES OR OTHER
+   LIABILITY, WHETHER IN AN ACTION OF CONTRACT, TORT OR OTHERWISE, ARISING FROM,
+   OUT OF OR IN CONNECTION WITH THE SOFTWARE OR THE USE OR OTHER DEALINGS IN THE
+   SOFTWARE.
+*)
+
+From stdpp Require Import base decidable gmap finite.
+From Coq Require Import ssreflect.
+From Coq.Program Require Import Equality.
+From Must Require Import gLts Bisimulation Lts_OBA Lts_FW Lts_OBA_FB StateTransitionSystems Termination
+    Must Bar CompletenessAS SoundnessAS Lift Subset_Act FiniteImageLTS WeakTransitions Convergence
+    InteractionBetweenLts MultisetLTSConstruction ForwarderConstruction  ParallelLTSConstruction ActTau
+    Testing_Predicate DefinitionAS DefinitionMS DefinitionFMS EquivalenceMS.
+
+Section failure_must_set.
+
+  Context `{P : Type}.
+  Context `{Q : Type}.
+  Context `{A : Type}.
+  Context `{H : !ExtAction A}.
+  Context `{gLtsP : !gLts P A, !FiniteImagegLts P A}.
+  Context `{gLtsQ : !gLts Q A, !FiniteImagegLts Q A}.
+
+  Context `{@gLtsObaFB P A H gLtsP gLtsEqP gLtsObaP}.
+  Context `{@gLtsObaFB Q A H gLtsQ gLtsEqQ gLtsObaQ}.
+
+  Context `{@Prop_of_Inter P (mb A) A fw_inter H gLtsP MbgLts}.
+  Context `{@Prop_of_Inter Q (mb A) A fw_inter H gLtsQ MbgLts}.
+
+  Lemma equivalence_must_set_nfailure
+    (p : P) (s : trace A) h1 (G : gset A) :
+    MUST__s (AFTER (p, ∅) s h1) G
+      <-> ¬ Failure (p, ∅) s G.
+  Proof.
+    split.
+    - intros hm (e & hw & hf). eassumption.
+      edestruct (hm e) as (μ & p' & mem' & hw'). eapply wt_set_spec2. eauto. eapply wt_nil.
+      edestruct (hf μ mem'). eauto.
+    - intros hnf.
+      assert (∀ p0 : P * mb A, p0 ∈ AFTER (p ▷ ∅) s h1 → p0 ⇓ []).
+      intros p0 mem0. eapply cnv_nil, cnv_wt_s_terminate; eauto.
+      eapply (wt_set_spec1 _ _ _ _ mem0).
+      destruct (either_MUST__s (AFTER (p, ∅) s h1) G) as [Hyp | Hyp]; eauto.
+      + eapply nMusts_ex in Hyp as (p0 & mem & hnm).
+        exfalso. eapply hnf.
+        eapply nMust_ex in hnm as (p1 & hw1 & hnp).
+        exists p1. split.
+        eapply wt_push_nil_right.
+        eapply (wt_set_spec1 _ _ _ _ mem). eassumption.
+        intros μ mem0 (p' & hw'). eapply hnp. eassumption.
+        eassumption.
+        eapply cnv_nil, cnv_wt_s_terminate; eauto.
+        eapply (wt_set_spec1 _ _ _ _ mem). eauto.
+  Qed.
+
+  Lemma equivalence_nmust_set_failure
+    (p : P) (s : trace A) h1 (G : gset A) :
+    ¬ MUST__s (AFTER (p ▷ ∅) s h1) G
+      <-> Failure (p ▷ ∅) s G.
+  Proof.
+    split.
+    - intro hm.
+      eapply nMusts_ex in hm as (p0 & mem & hnm).
+      eapply nMust_ex in hnm as (p1 & hw1 & hnp).
+      exists p1. split.
+      eapply wt_push_nil_right.
+      eapply (wt_set_spec1 _ _ _ _ mem). eassumption.
+      intros μ mem0 (p' & hw'). eapply hnp. eassumption.
+      eassumption.
+      eapply cnv_nil, cnv_wt_s_terminate; eauto.
+      eapply (wt_set_spec1 _ _ _ _ mem).
+      intros p0 mem0. eapply cnv_nil, cnv_wt_s_terminate; eauto.
+      eapply (wt_set_spec1 _ _ _ _ mem0).
+    - intros (e & hmem & hf) hm. eassumption.
+      unfold MUST__s in hm.
+      unfold MUST in hm.
+      edestruct (hm e) as (μ & p1 & mem1 & hw1).
+      eapply (wt_set_spec2 _ _ _ _ hmem). eapply wt_nil.
+      eapply (hf μ mem1). eauto.
+  Qed.
+
+End failure_must_set.
+
+Section failure_must_set_pre.
+  Context `{P : Type}.
+  Context `{Q : Type}.
+  Context `{A : Type}.
+  Context `{H : !ExtAction A}.
+  Context `{gLtsP : !gLts P A, !FiniteImagegLts P A}.
+  Context `{gLtsQ : !gLts Q A, !FiniteImagegLts Q A}.
+
+  Context `{@gLtsObaFB P A H gLtsP gLtsEqP gLtsObaP}.
+  Context `{@gLtsObaFB Q A H gLtsQ gLtsEqQ gLtsObaQ}.
+
+  Context `{@Prop_of_Inter P (mb A) A fw_inter H gLtsP MbgLts}.
+  Context `{@Prop_of_Inter Q (mb A) A fw_inter H gLtsQ MbgLts}.
+
+  Theorem equivalence_pre_failure_must_set
+
+  (p : P) (q : Q) : (p ▷ ∅) ≾ (q ▷ ∅) <-> (p ▷ ∅) ⋖ (q ▷ ∅).
+  Proof.
+    split.
+    - intros (hpre1 & hpre2). split.
+      + exact hpre1.
+      + intros s G hf hcnv.
+        eapply (equivalence_nmust_set_failure p s hcnv).
+        intros hm. eapply (hpre2 s hcnv (hpre1 s hcnv)) in hm.
+        eapply (equivalence_must_set_nfailure q s (hpre1 s hcnv) G) in hm. contradiction. eassumption.
+    - intros (hpre1 & hpre2). split. 
+      + exact hpre1. 
+      + intros s h1 h2 G hm%equivalence_must_set_nfailure.
+        eapply (equivalence_must_set_nfailure q).
+        intros hf%hpre2. contradiction.
+  Qed.
+
+End failure_must_set_pre.
+
