theories/Testing_Pre_orders/Must/Alternative_Preorder/Must_Set/DefinitionMS.v
@@ -1,0 +1,71 @@
+(*
+   Copyright (c) 2024 Nomadic Labs
+   Copyright (c) 2024 Paul Laforgue <paul.laforgue@nomadic-labs.com>
+   Copyright (c) 2024 Léo Stefanesco <leo.stefanesco@mpi-sws.org>
+   Copyright (c) 2025 Gaëtan Lopez <glopez@irif.fr>
+
+   Permission is hereby granted, free of charge, to any person obtaining a copy
+   of this software and associated documentation files (the "Software"), to deal
+   in the Software without restriction, including without limitation the rights
+   to use, copy, modify, merge, publish, distribute, sublicense, and/or sell
+   copies of the Software, and to permit persons to whom the Software is
+   furnished to do so, subject to the following conditions:
+
+   The above copyright notice and this permission notice shall be included in all
+   copies or substantial portions of the Software.
+
+   THE SOFTWARE IS PROVIDED "AS IS", WITHOUT WARRANTY OF ANY KIND, EXPRESS OR
+   IMPLIED, INCLUDING BUT NOT LIMITED TO THE WARRANTIES OF MERCHANTABILITY,
+   FITNESS FOR A PARTICULAR PURPOSE AND NONINFRINGEMENT. IN NO EVENT SHALL THE
+   AUTHORS OR COPYRIGHT HOLDERS BE LIABLE FOR ANY CLAIM, DAMAGES OR OTHER
+   LIABILITY, WHETHER IN AN ACTION OF CONTRACT, TORT OR OTHERWISE, ARISING FROM,
+   OUT OF OR IN CONNECTION WITH THE SOFTWARE OR THE USE OR OTHER DEALINGS IN THE
+   SOFTWARE.
+*)
+
+From Coq.Unicode Require Import Utf8.
+From Coq.Program Require Import Equality.
+From stdpp Require Import finite gmap decidable.
+From Must Require Import ActTau gLts Bisimulation Lts_OBA Subset_Act WeakTransitions Testing_Predicate
+    StateTransitionSystems InteractionBetweenLts Convergence Termination FiniteImageLTS.
+
+Section must_sets.
+
+  (* https://arxiv.org/pdf/1612.03191.pdf *)
+
+  Local Open Scope positive.
+
+  Definition MUST `{gLts P A} 
+    (p : P) (G : gset A) :=
+    forall p', p ⟹ p' -> exists μ p0, μ ∈ G /\ p' ⟹{μ} p0.
+
+  Definition MUST__s `{FiniteImagegLts P A} 
+    (ps : gset P) (G : gset A) := 
+    forall p, p ∈ ps -> MUST p G.
+
+  (* Residuals of a process p AFTER the execution of s. *)
+
+  Definition AFTER `{FiniteImagegLts P A} 
+    (p : P) (s : trace A) (hcnv : p ⇓ s) := 
+    wt_set p s hcnv. 
+
+  Definition bhv_pre_ms_cond1 `{gLts P A, gLts Q A} 
+  (p : P) (q : Q) := forall s, p ⇓ s -> q ⇓ s.
+
+  Definition bhv_pre_ms_cond2 `{@FiniteImagegLts P A H gLtsP, @FiniteImagegLts Q A H gLtsQ} 
+    (p : P) (q : Q) :=
+    forall s h1 h2 G, MUST__s (AFTER p s h1) G -> MUST__s (AFTER q s h2) G.
+
+  Definition bhv_pre_ms `{@FiniteImagegLts P A H gLtsP, @FiniteImagegLts Q A H gLtsQ} 
+    (p : P) (q : Q) :=
+    bhv_pre_ms_cond1 p q /\ bhv_pre_ms_cond2 p q.
+End must_sets.
+
+Global Hint Unfold bhv_pre_ms:mdb.
+
+Notation "p ≾₁ q" := (bhv_pre_ms_cond1 p q) (at level 70).
+
+Notation "p ≾₂ q" := (bhv_pre_ms_cond2 p q) (at level 70).
+
+Notation "p ≾ q" := (bhv_pre_ms p q) (at level 70).
+
