theories/Testing_Pre_orders/Must/Alternative_Preorder/Must_Set/Equivalence/CompletenessMS.v
@@ -1,0 +1,38 @@
+(*
+   Copyright (c) 2024 Nomadic Labs
+   Copyright (c) 2024 Paul Laforgue <paul.laforgue@nomadic-labs.com>
+   Copyright (c) 2024 Léo Stefanesco <leo.stefanesco@mpi-sws.org>
+   Copyright (c) 2025 Gaëtan Lopez <glopez@irif.fr>
+
+   Permission is hereby granted, free of charge, to any person obtaining a copy
+   of this software and associated documentation files (the "Software"), to deal
+   in the Software without restriction, including without limitation the rights
+   to use, copy, modify, merge, publish, distribute, sublicense, and/or sell
+   copies of the Software, and to permit persons to whom the Software is
+   furnished to do so, subject to the following conditions:
+
+   The above copyright notice and this permission notice shall be included in all
+   copies or substantial portions of the Software.
+
+   THE SOFTWARE IS PROVIDED "AS IS", WITHOUT WARRANTY OF ANY KIND, EXPRESS OR
+   IMPLIED, INCLUDING BUT NOT LIMITED TO THE WARRANTIES OF MERCHANTABILITY,
+   FITNESS FOR A PARTICULAR PURPOSE AND NONINFRINGEMENT. IN NO EVENT SHALL THE
+   AUTHORS OR COPYRIGHT HOLDERS BE LIABLE FOR ANY CLAIM, DAMAGES OR OTHER
+   LIABILITY, WHETHER IN AN ACTION OF CONTRACT, TORT OR OTHERWISE, ARISING FROM,
+   OUT OF OR IN CONNECTION WITH THE SOFTWARE OR THE USE OR OTHER DEALINGS IN THE
+   SOFTWARE.
+*)
+
+From Coq Require ssreflect Setoid.
+From Coq.Unicode Require Import Utf8.
+From Coq.Lists Require Import List.
+Import ListNotations.
+From Coq.Program Require Import Wf Equality.
+From Coq.Wellfounded Require Import Inverse_Image.
+From Coq.Logic Require Import JMeq ProofIrrelevance.
+From stdpp Require Import sets base countable finite gmap list finite decidable finite gmap.
+From Must Require Import gLts Bisimulation Lts_OBA WeakTransitions Lts_OBA_FB Lts_FW FiniteImageLTS
+      InteractionBetweenLts MultisetLTSConstruction ParallelLTSConstruction ForwarderConstruction
+       Must Lift Subset_Act Convergence Termination Testing_Predicate DefinitionAS DefinitionMS.
+From Must Require Import ActTau.
+
