theories/Testing_Pre_orders/Must/Alternative_Preorder/Must_Set/Equivalence/EquivalenceMS.v
@@ -1,0 +1,286 @@
+(*
+   Copyright (c) 2024 Nomadic Labs
+   Copyright (c) 2024 Paul Laforgue <paul.laforgue@nomadic-labs.com>
+   Copyright (c) 2024 Léo Stefanesco <leo.stefanesco@mpi-sws.org>
+   Copyright (c) 2025 Gaëtan Lopez <glopez@irif.fr>
+
+   Permission is hereby granted, free of charge, to any person obtaining a copy
+   of this software and associated documentation files (the "Software"), to deal
+   in the Software without restriction, including without limitation the rights
+   to use, copy, modify, merge, publish, distribute, sublicense, and/or sell
+   copies of the Software, and to permit persons to whom the Software is
+   furnished to do so, subject to the following conditions:
+
+   The above copyright notice and this permission notice shall be included in all
+   copies or substantial portions of the Software.
+
+   THE SOFTWARE IS PROVIDED "AS IS", WITHOUT WARRANTY OF ANY KIND, EXPRESS OR
+   IMPLIED, INCLUDING BUT NOT LIMITED TO THE WARRANTIES OF MERCHANTABILITY,
+   FITNESS FOR A PARTICULAR PURPOSE AND NONINFRINGEMENT. IN NO EVENT SHALL THE
+   AUTHORS OR COPYRIGHT HOLDERS BE LIABLE FOR ANY CLAIM, DAMAGES OR OTHER
+   LIABILITY, WHETHER IN AN ACTION OF CONTRACT, TORT OR OTHERWISE, ARISING FROM,
+   OUT OF OR IN CONNECTION WITH THE SOFTWARE OR THE USE OR OTHER DEALINGS IN THE
+   SOFTWARE.
+*)
+
+From stdpp Require Import base decidable gmap finite.
+From Coq Require Import ssreflect.
+From Coq.Program Require Import Equality.
+From Must Require Import gLts Bisimulation Lts_OBA Lts_FW Lts_OBA_FB StateTransitionSystems Termination
+    Must Bar CompletenessAS SoundnessAS Lift Subset_Act FiniteImageLTS WeakTransitions Convergence
+    InteractionBetweenLts MultisetLTSConstruction ForwarderConstruction ParallelLTSConstruction ActTau
+    Testing_Predicate DefinitionAS DefinitionMS MustE.
+
+Section must_set_acc_set.
+  Context `{P : Type}.
+  Context `{Q : Type}.
+  Context `{A : Type}.
+  Context `{H : !ExtAction A}.
+  Context `{gLtsP : !gLts P A, !FiniteImagegLts P A}.
+  Context `{gLtsQ : !gLts Q A, !FiniteImagegLts Q A}.
+
+  Context `{@gLtsObaFB P A H gLtsP gLtsEqP gLtsObaP}.
+  Context `{@gLtsObaFB Q A H gLtsQ gLtsEqQ gLtsObaQ}.
+
+  Context `{@Prop_of_Inter P (mb A) A fw_inter H gLtsP MbgLts}.
+  Context `{@Prop_of_Inter Q (mb A) A fw_inter H gLtsQ MbgLts}.
+
+(*   Definition actions_acc 
+  (p : P * mb A) s (h : p ⇓ s) : gset PreA := oas p s h. *)
+
+  (* ************************************************** *)
+
+  Lemma either_wperform_mu 
+  (p : P * mb A) μ :
+    p ⤓ -> (exists q, p ⟹{μ} q) \/ ~ (exists q, p ⟹{μ} q).
+  Proof.
+    intro ht. induction ht.
+    destruct (lts_refuses_decidable p (ActExt μ)).
+    - assert (∀ x, x ∈ enum (dsig (lts_step p τ)) -> (∃ q0, `x ⟹{μ} q0) \/ ~ (∃ q0, `x ⟹{μ} q0))
+         as Hyp
+        by (intros (x & mem) _; set_solver).
+      edestruct (exists_forall_in _ _ _ Hyp) as [Hyp' | Hyp'].
+      + eapply Exists_exists in Hyp' as ((q' & pr) & mem & (q0 & hw)).
+        left. exists q0. eapply wt_tau; eauto. now eapply bool_decide_unpack.
+      + right. intros (q' & hw). inversion hw; subst.
+        ++ contradict Hyp'. intros n. rewrite Forall_forall in n.
+           eapply (n (dexist q l0)). eapply elem_of_enum. eauto.
+        ++ eapply (@lts_refuses_spec2 (P * mb A)); eauto.
+    - left. eapply lts_refuses_spec1 in n as (q & l). eauto with mdb.
+  Qed.
+
+  Lemma either_wperform_mem (p : P * mb A) (G : gset A) (ht : p ⤓) :
+    (exists μ p', μ ∈ G /\ p ⟹{μ} p') 
+      \/ (forall μ p', μ ∈ G -> ~ p ⟹{μ} p').
+  Proof.
+    induction G using set_ind_L; [|destruct IHG, (either_wperform_mu p x)]; set_solver.
+  Qed.
+
+  Lemma either_wperform_mem_set
+    (ps : gset (P * mb A)) (G : gset A) (ht : forall p, p ∈ ps -> p ⤓) :
+    (exists p', p' ∈ ps /\ forall μ p0, μ ∈ G
+      -> ~ p' ⟹{μ} p0) 
+      \/ (forall p', p' ∈ ps -> exists μ p0, μ ∈ G /\ p' ⟹{μ} p0).
+  Proof.
+    induction ps using set_ind_L. 
+    + set_solver. 
+    + destruct IHps, (@either_wperform_mem x G); set_solver.
+  Qed.
+
+  Lemma either_MUST
+      (p : P * mb A) (G : gset A) (hcnv : p ⇓ []) :
+      MUST p G \/ ~ MUST p G.
+  Proof.
+    assert (∀ p0 : P * mb A, p0 ∈ wt_set p [] hcnv → p0 ⤓) as pre_Hyp.
+    intros p0 mem0%wt_set_spec1. eapply cnv_terminate, cnv_preserved_by_wt_nil; eauto.
+    destruct (either_wperform_mem_set (wt_set p [] hcnv) G) 
+      as [Hyp|]; eauto.
+    - right. intro hm. destruct Hyp as (p' & mem%wt_set_spec1%hm & nhw). set_solver.
+    - left. intros p1 hw%(wt_set_spec2 _ p1 [] hcnv). set_solver.
+  Qed.
+
+  Lemma either_ex_nMUST_or_MUST
+    (ps : gset (P * mb A)) (G : gset A)
+      (ht : forall p, p ∈ ps -> p ⇓ []) :
+    (exists p, p ∈ ps /\ ~ MUST p G) 
+      \/ (forall p, p ∈ ps -> MUST p G).
+  Proof.
+    induction ps using set_ind_L; [|edestruct IHps, (either_MUST x G)]; set_solver.
+  Qed.
+
+  Lemma either_MUST__s
+    (ps : gset (P * mb A)) (G : gset A)  :
+    (forall p, p ∈ ps -> p ⇓ []) -> MUST__s ps G \/ ~ MUST__s ps G.
+  Proof.
+    intros. edestruct (either_ex_nMUST_or_MUST ps G) as [Hyp |]; eauto.
+    right. intros hm. destruct Hyp as (p0 & mem0%hm & hnm). contradiction.
+  Qed.
+
+  Lemma nMusts_ex
+    (ps : gset (P * mb A)) (G : gset A) :
+    (forall p, p ∈ ps -> p ⇓ []) -> ~ MUST__s ps G 
+    -> exists p, p ∈ ps /\ ~ MUST p G.
+  Proof. intros. edestruct (either_ex_nMUST_or_MUST ps G); set_solver. Qed.
+
+  Lemma nMust_ex
+    (p : P * mb A) (G : gset A) (hcnv : p ⇓ []) 
+    (hnm : ~ MUST p G) :
+    exists p', p ⟹ p' /\ forall μ p0, μ ∈ G -> ~ p' ⟹{μ} p0.
+  Proof.
+    assert (∀ p0 : P * mb A, p0 ∈ wt_set p [] hcnv → p0 ⤓).
+    intros p0 mem0%wt_set_spec1. eapply cnv_terminate, cnv_preserved_by_wt_nil; eauto.
+    destruct (either_wperform_mem_set (wt_set p [] hcnv) G) as [Hyp|Hyp]; eauto.
+    - destruct Hyp as (p' & mem'%wt_set_spec1 & nhw). set_solver.
+    - edestruct hnm. intros p' mem. eapply Hyp. eapply wt_set_spec2; eauto.
+  Qed.
+
+  Lemma nMusts_nMust
+  (p : P * mb A) (G : gset A) (hcnv : p ⇓ []) 
+  (hnm : ~ MUST__s (wt_set p [] hcnv) G) : 
+  ¬ MUST p G.
+  Proof.
+    intro hm. eapply hnm. intros p' mem0%wt_set_spec1.
+    intros r hw. eapply hm. eapply wt_push_nil_left; eassumption.
+  Qed.
+
+(*   Lemma nMust_out_acc_ex 
+
+    (p : P * mb A) pt G s hcnv :
+
+    pt ∈ AFTER p s hcnv 
+    -> ~ MUST pt (union_of_actions_without ((elements (wt_refuses_set p s hcnv)) , q')) ->
+    exists p', pt ⟹ p' /\ p' ↛ /\ lts_acc_set_of p' ⊆ lts_acc_set_of q'.
+  Proof.
+    intros mem%wt_set_spec1 hnm.
+    eapply nMust_ex in hnm as (p' & hw' & nhw).
+    assert (ht': p' ⤓)
+      by (eapply (cnv_wt_s_terminate p p' s hcnv), wt_push_nil_right; eauto).
+    eapply terminate_then_wt_refuses in ht' as (p0 & hw0 & hst).
+    exists p0. split. eapply wt_push_nil_left; eauto.
+    split; eauto.
+    intros μ mem_mu.
+    assert (mem0 : μ ∈ actions_acc p s hcnv).
+    eapply elem_of_union_list. eexists. split; eauto.
+    eapply elem_of_list_fmap.
+    exists p0. repeat split; eauto.
+    eapply elem_of_elements, wt_refuses_set_spec2; split; eauto.
+    eapply wt_push_nil_right, wt_push_nil_right; eauto.
+    eapply lts_refuses_spec1 in mem_mu as (p'0 & HypTr).
+    { destruct (decide (μ ∈ lts_acc_set_of q')).
+      + eauto.
+      + exfalso.
+        eapply (nhw $ μ); eauto. unfold actions_acc in mem0.
+        unfold oas in mem0. set_solver.
+        eapply wt_push_nil_left; eauto with mdb. }
+    constructor; eapply (cnv_wt_s_terminate p pt s hcnv); eauto.
+  Qed. *)
+
+(*   Lemma either_MUST_or_ex 
+    (p : P * mb A) (q' : Q * mb A)  s hcnv :
+    MUST__s (AFTER p s hcnv) (union_of_actions_without ((elements (wt_refuses_set p s hcnv)) , q'))
+    \/ (exists p', p ⟹[s] p' /\ p' ↛ /\ lts_acc_set_of p' ⊆ lts_acc_set_of q').
+  Proof.
+    assert (h1 : forall p0, p0 ∈ AFTER p s hcnv → p0 ⇓ []).
+    intros p0 mem0. eapply cnv_nil, cnv_wt_s_terminate; eauto.
+    eapply (wt_set_spec1 _ _ _ _ mem0).
+    destruct (either_MUST__s (AFTER p s hcnv) ((elements (wt_refuses_set p s hcnv)) , q')) 
+        as [ |Hyp].
+    + eauto.
+    + left. eauto.
+    + right.
+      eapply nMusts_ex in Hyp as (pt & mem & hnm); eauto.
+      eapply nMust_out_acc_ex in hnm as (pt' & hw & hst & hsub); eauto.
+      exists pt'. split; eauto. eapply wt_push_nil_right; eauto. now eapply wt_set_spec1 in mem.
+  Qed. *)
+
+(*   Lemma Must_out_acc_npre 
+    (p : P * mb A) (q q' : Q * mb A) s hcnv :
+    q ⇓ s -> q ⟹[s] q' -> q' ↛ ->
+    MUST__s (AFTER p s hcnv) (actions_acc p s hcnv ∖ lts_acc_set_of q') ->
+    ~ p ≾₂ q.
+  Proof.
+    intros hcnv' hw hst hm pre2.
+    set (G := actions_acc p s hcnv ∖ lts_acc_set_of q').
+    assert (exists μ t, μ ∈ G /\ q' ⟹{μ} t) as (μ & t & mem & hw').
+    eapply (pre2 s hcnv hcnv'); eauto. eapply wt_set_spec2; eauto. eapply wt_nil.
+    eapply elem_of_difference in mem as (mem & nmem).
+    (* assert (exists p', p' ⟶[ μ ]).
+    assert (is_output μ) as (a & heq). *)
+    eapply elem_of_union_list in mem as (X & mem1 & mem2).
+    eapply elem_of_list_fmap in mem1 as (r & heq & mem1). subst.
+    (* eapply elem_of_map in mem2 as (a & heq & mem2). exists a. assumption. *)
+    assert { r' | r ⟶[ μ ] r'} as (r' & HypTr). eapply lts_refuses_spec1. eauto.
+    inversion hw'; subst.
+    eapply lts_refuses_spec2 in hst; eauto.
+    eapply nmem. eapply lts_refuses_spec2. eauto.
+  Qed. *)
+
+  (* ************************************************** *)
+
+  Context `{@PreExtAction A H (P * mb A) FinA PreA PreA_eq PreA_countable 𝝳 Φ (FW_gLts gLtsP)}.
+  Context `{@PreExtAction A H (Q * mb A) FinA PreA PreA_eq PreA_countable 𝝳 Φ (FW_gLts gLtsQ)}.
+
+  Lemma equivalence_bhv_acc_mst2
+    (p : P) (q : Q) :
+    (p, ∅) ≼₁ (q, ∅) -> (p, ∅) ≾₂ (q, ∅) <-> (p, ∅) ≼₂ (q, ∅).
+  Proof.
+    intro hpre1.
+    split.
+    - intro hpre2. intros s q' hcnv hw hst.
+      (* edestruct (either_MUST_or_ex (p, ∅) q' s hcnv).
+      + exfalso. eapply Must_out_acc_npre; eauto with mdb.
+      + set_solver. *) admit.
+    - intro hpre2.
+      intros s hcnv hcnv' G hm q' mem%wt_set_spec1 q0 hw.
+      assert (exists r, q0 ⟹ r /\ r ↛) as (qt & hw' & hstq').
+      { eapply terminate_then_wt_refuses, terminate_preserved_by_wt_nil; eauto.
+        eapply cnv_wt_s_terminate; eauto. }
+      edestruct (hpre2 s qt hcnv) as (pt & hwpt & hstpt & hsubpt); eauto.
+      eapply wt_push_nil_right; eauto. eapply wt_push_nil_right; eauto.
+      assert (exists μ r, μ ∈ G /\ pt ⟹{μ} r) as (μ & p0 & mem0 & hw0).
+      { eapply hm. eapply wt_set_spec2; eauto. eapply wt_nil. }
+      exists μ. inversion hw0; subst.
+      + exfalso. eapply lts_refuses_spec2 in hstpt; eauto.
+      + assert (𝝳 (Φ μ) ∈ pre_co_actions_of qt).
+        { eapply hsubpt. eapply preactions_of_spec. eapply preactions_of_fin_test_spec1.
+          admit. }
+        (* exists qr. split; eauto. eapply wt_push_nil_left; eauto with mdb. *)
+        admit.
+  Admitted.
+
+  Theorem equivalence_bhv_acc_mst
+  (p : P) (q : Q) :
+  (p, ∅) ≾ (q, ∅) <-> (p, ∅) ≼ (q, ∅).
+  Proof.
+    split; intros (pre1 & pre2); split; eauto; now eapply equivalence_bhv_acc_mst2.
+  Qed.
+
+  Context `{attaboy : E -> Prop}.
+  Context `{attaboy_dec : forall e, Decision (attaboy e)}.
+  Context `{gLtsE : !gLts E A, !FiniteImagegLts E A, gLtsEqE: !gLtsEq E A, !Testing_Predicate E A attaboy}.
+  Context `{@Prop_of_Inter P E A parallel_inter H gLtsP gLtsE}.
+  Context `{@Prop_of_Inter Q E A parallel_inter H gLtsQ gLtsE}.
+
+  Context `{@gLtsObaFB E A H gLtsE gLtsEqE gLtsObaE}.
+
+  Context `{@Prop_of_Inter (P * mb A) E A parallel_inter H (inter_lts fw_inter) gLtsE}.
+  Context `{@Prop_of_Inter (Q * mb A) E A parallel_inter H (inter_lts fw_inter) gLtsE}.
+
+  Context `{@PreExtAction A H (P * mb A) FinA PreA PreA_eq PreA_countable 𝝳 Φ (FW_gLts gLtsP)}.
+  Context `{@PreExtAction A H (Q * mb A) FinA PreA PreA_eq PreA_countable 𝝳 Φ (FW_gLts gLtsQ)}.
+  Context `{@AbsAction A H E FinA gLtsE Φ}.
+
+  Context `{igen_conv : @gen_spec_conv E _ _ _ _ attaboy Testing_Predicate0 co_of gen_conv}.
+  Context `{igen_acc : @gen_spec_acc PreA _ _ E _ _ _ _ attaboy Testing_Predicate0 co_of gen_acc (fun x => 𝝳 (Φ x))}.
+
+  Corollary equivalence_bhv_mst_ctx
+    (p : P) (q : Q) : (p, ∅) ≾ (q, ∅) <-> @pre_extensional P Q _ _ _ attaboy _ p q.
+  Proof.
+    erewrite pre_extensional_eq.
+    rewrite equivalence_bhv_acc_mst.
+    rewrite <- equivalence_bhv_acc_ctx.
+    eapply pre_extensional_eq.
+  Qed.
+
+
+End must_set_acc_set.
