theories/Testing_Pre_orders/Must/Application/Application.v
@@ -1,0 +1,260 @@
+(*
+   Copyright (c) 2024 Nomadic Labs
+   Copyright (c) 2024 Paul Laforgue <paul.laforgue@nomadic-labs.com>
+   Copyright (c) 2024 Léo Stefanesco <leo.stefanesco@mpi-sws.org>
+   Copyright (c) 2025 Gaëtan Lopez <glopez@irif.fr>
+
+   Permission is hereby granted, free of charge, to any person obtaining a copy
+   of this software and associated documentation files (the "Software"), to deal
+   in the Software without restriction, including without limitation the rights
+   to use, copy, modify, merge, publish, distribute, sublicense, and/or sell
+   copies of the Software, and to permit persons to whom the Software is
+   furnished to do so, subject to the following conditions:
+
+   The above copyright notice and this permission notice shall be included in all
+   copies or substantial portions of the Software.
+
+   THE SOFTWARE IS PROVIDED "AS IS", WITHOUT WARRANTY OF ANY KIND, EXPRESS OR
+   IMPLIED, INCLUDING BUT NOT LIMITED TO THE WARRANTIES OF MERCHANTABILITY,
+   FITNESS FOR A PARTICULAR PURPOSE AND NONINFRINGEMENT. IN NO EVENT SHALL THE
+   AUTHORS OR COPYRIGHT HOLDERS BE LIABLE FOR ANY CLAIM, DAMAGES OR OTHER
+   LIABILITY, WHETHER IN AN ACTION OF CONTRACT, TORT OR OTHERWISE, ARISING FROM,
+   OUT OF OR IN CONNECTION WITH THE SOFTWARE OR THE USE OR OTHER DEALINGS IN THE
+   SOFTWARE.
+*)
+
+From stdpp Require Import base decidable gmap finite.
+From Coq Require Import ssreflect.
+From Coq.Program Require Import Equality.
+From Must Require Import gLts Bisimulation Lts_OBA Lts_FW Lts_OBA_FB StateTransitionSystems Termination
+    Must Bar CompletenessAS SoundnessAS Lift Subset_Act FiniteImageLTS WeakTransitions Convergence
+    InteractionBetweenLts MultisetLTSConstruction ForwarderConstruction  ParallelLTSConstruction ActTau
+    Testing_Predicate DefinitionAS MustE EquivalenceAS.
+From stdpp Require Import gmultiset.
+
+Section application.
+
+  Lemma nil_refuses
+  {Q A : Type} {H : ExtAction A}
+  `{@gLtsOba Q A H gLtsQ gLtsEqQ}
+  `{@Prop_of_Inter Q (mb A) A fw_inter H gLtsQ MbgLts}
+
+  (q : Q) (h : forall α, q ↛{α}) (m : mb A) : 
+  lts_refuses (q, m) τ.
+  Proof.
+    destruct (decide ((q, m) ↛)); eauto.
+    eapply lts_refuses_spec1 in n as (q' & l').
+    inversion l'; subst.
+    + edestruct lts_refuses_spec2; eauto.
+    + inversion l.
+    + edestruct lts_refuses_spec2; eauto.
+  Qed.
+
+  Lemma nil_cnv
+  {Q A : Type} {H : ExtAction A}
+  `{@gLtsOba Q A H gLtsQ gLtsEqQ}
+  `{@Prop_of_Inter Q (mb A) A fw_inter H gLtsQ MbgLts}
+  (q : Q) (h : forall α, q ↛{α}) s m : 
+  (q, m) ⇓ s.
+  Proof.
+    dependent induction s.
+    - now eapply cnv_nil, terminate_if_refuses, nil_refuses.
+    - eapply cnv_act.
+      + now eapply terminate_if_refuses, nil_refuses.
+      + intros (q', m') hw. inversion hw; subst.
+        ++ exfalso. eapply (@lts_refuses_spec2 (Q * mb A)).
+           eauto. now eapply nil_refuses.
+        ++ inversion l; subst.
+           +++ edestruct lts_refuses_spec2. eauto. eauto.
+           +++ eapply cnv_preserved_by_wt_nil; eauto.
+  Qed.
+
+  CoInductive ionly_spec {P A : Type} {H : ExtAction A} 
+    `{@gLtsOba P A H gLtsQ gLtsEqQ} (p : P) : Prop :=
+  | mstep : (forall μ p', p ⟶[μ] p' -> exist_co_nba μ) 
+        -> (forall α p', p ⟶{α} p' -> ionly_spec p') -> ionly_spec p.
+
+  Lemma lts_non_blocking_ionly_spec {P A : Type}
+        `{gLtsOba P A} (p : P) (pr : ionly_spec p) : dom (lts_oba_mo p) = ∅.
+  Proof.
+    eapply leibniz_equiv. intro a. split.
+    + intros mem.
+      eapply gmultiset_elem_of_dom in mem.
+      eapply lts_oba_mo_spec_bis2 in mem as (p' & nb & l').
+      destruct pr as (h1 & h2). eapply h1 in l' as (a' & nb' & duo').
+      eapply dual_blocks in nb'; eauto.
+      contradiction.
+    + intro. set_solver.
+Qed.
+
+  Lemma lts_non_blocking_ionly_spec_wt_nil_empty_mb 
+    {Q A : Type} {H : ExtAction A}
+    `{M : @gLtsObaFB Q A H gLtsQ gLtsEqQ gLtsObaQ}
+    `{@Prop_of_Inter Q (mb A) A fw_inter H gLtsQ MbgLts}
+    p (pr : ionly_spec p) :
+    (p, ∅) ⤓ -> forall t, (p, ∅) ⟹ t -> dom (lts_oba_mo t) = ∅.
+  Proof.
+    intros hpt p' hw.
+    dependent induction hpt. dependent induction hw.
+    - simpl.
+      assert (disj_union (lts_oba_mo p) empty = (lts_oba_mo p)) as eq.
+      multiset_solver. rewrite eq.
+      now eapply lts_non_blocking_ionly_spec.
+    - inversion l; subst.
+      + destruct pr as (h1 & h2). eapply H2; eauto.
+      + inversion l0.
+      + exfalso. eapply (gmultiset_not_elem_of_empty μ2).
+        assert (non_blocking μ2) as nb.
+        destruct eq; eauto.
+        eapply non_blocking_action_in_ms in nb; eauto.
+        replace (∅ : gmultiset A) with ({[+ μ2 +]} ⊎ b2) by eauto. multiset_solver.
+    Qed.
+
+  Lemma lts_non_blocking_ionly_spec_wt_nil 
+    {Q A : Type} {H : ExtAction A}
+    `{M : @gLtsObaFB Q A H gLtsQ gLtsEqQ gLtsObaQ}
+    `{@Prop_of_Inter Q (mb A) A fw_inter H gLtsQ MbgLts}
+    n p (pr : ionly_spec p) m :
+    (p, m) ⤓ -> size m = n -> forall t, (p, m) ⟹ t
+      -> dom (lts_oba_mo t) ⊆ dom m.
+  Proof.
+    dependent induction n; subst; intro hpt; dependent induction hpt; intros heq p' hw.
+    - eapply gmultiset_size_empty_inv in heq. subst.
+      replace (dom (lts_oba_mo p')) with (∅ : gset A).
+      + multiset_solver. 
+      + symmetry. eapply lts_non_blocking_ionly_spec_wt_nil_empty_mb; eauto with mdb.
+    - inversion hw; subst.
+      + simpl. 
+        intro μ. intro mem.
+        eapply gmultiset_elem_of_dom in mem.
+        eapply gmultiset_elem_of_disj_union in mem.
+        destruct mem as [in_oba | in_mem].
+        ++ eapply gmultiset_elem_of_dom. eapply gmultiset_elem_of_dom in in_oba.
+           eapply lts_non_blocking_ionly_spec in pr.
+           set_solver.
+        ++ eapply gmultiset_elem_of_dom.
+           eapply lts_mb_nb_with_nb_spec1 in in_mem as (nb & in_mem).
+           exact in_mem.
+      + destruct pr as (h1 & h2); inversion l; subst; eauto.
+        ++ inversion l0.
+        ++ assert (non_blocking μ2) as nb. destruct eq; eauto.
+           eapply non_blocking_action_in_ms in nb; eauto; subst.
+           eapply IHn in w; eauto with mdb.
+           +++ intros b mem%w%gmultiset_elem_of_dom.
+               eapply gmultiset_elem_of_dom.
+               multiset_solver.
+           +++ rewrite gmultiset_size_disj_union in heq. 
+               rewrite gmultiset_size_singleton in heq. eauto.
+  Qed.
+
+  Lemma ionly_nil_leq2_wt_nil 
+    {Q A : Type} {H : ExtAction A}
+    `{M : @gLtsObaFB Q A H gLtsQ gLtsEqQ gLtsObaQ}
+    `{@Prop_of_Inter Q (mb A) A fw_inter H gLtsQ MbgLts}
+    n p (pr : ionly_spec p) m :
+    (p, m) ⤓ -> size m = n -> exists t, (p, m) ⟹ t /\ t ↛ /\ dom (lts_oba_mo t) ⊆ dom m.
+  Proof.
+    intros ht heq. edestruct @terminate_then_wt_refuses as (t & hw & hst); eauto with mdb.
+    exists t; split; eauto. split; eauto. eapply lts_non_blocking_ionly_spec_wt_nil; eauto.
+  Qed.
+
+  Lemma ionly_wt
+    {Q A : Type} {H : ExtAction A}
+    `{M : @gLtsOba Q A H gLtsQ gLtsEqQ}
+    `{@Prop_of_Inter Q (mb A) A fw_inter H gLtsQ MbgLts}
+    p (pr : ionly_spec p) m p' m' : 
+    (p ▷ m) ⟹ (p' ▷ m') 
+      -> ionly_spec p'.
+  Proof.
+    intro mem.
+    dependent induction mem.
+    + exact pr.
+    + inversion l; subst.
+      ++ destruct pr as (only_receive & Hyp). assert (ionly_spec a2).
+         eapply Hyp; eauto. eapply IHmem; eauto.
+      ++ inversion l0.
+      ++ destruct eq as (nb & duo).
+         assert (ionly_spec a2). destruct pr as (only_receive & Hyp).
+         eapply Hyp; eauto. eapply IHmem; eauto.
+  Qed.
+
+ (*  Lemma ionly_nil_leq2 {P Q A : Type} `{
+    @gLtsObaFB P A H gLtsP gLtsEqP gLtsObaP,
+    @gLtsObaFB Q A H gLtsQ gLtsEqQ gLtsObaQ}
+
+    `{@Prop_of_Inter P (mb A) A fw_inter H gLtsP MbgLts}
+    `{@Prop_of_Inter Q (mb A) A fw_inter H gLtsQ MbgLts}
+
+    (p : P) (pr : ionly_spec p) (q : Q) m (h : forall α, q ↛{α}) : 
+    (p, m) ≼₂ (q, m).
+  Proof.
+    intros s t hcnv hw hst.
+    dependent induction hw.
+    - inversion hcnv; subst.
+      edestruct ionly_nil_leq2_wt_nil as (p' & hw & hst' & hsub); eauto.
+      exists p'. split; eauto.
+      split; eauto.
+      intro μ. intro mem.
+      destruct (decide (non_blocking μ)) as [nb | not_nb].
+      + rename μ into η.
+        eapply lts_refuses_spec1 in mem as (p'' & Tr).
+        assert (η ∈ dom (lts_oba_mo p')) as mem'.
+        eapply gmultiset_elem_of_dom. eapply lts_oba_mo_spec_bis1; eauto.
+        eapply hsub in mem'. eapply lts_refuses_spec2.
+        eapply gmultiset_elem_of_dom in mem'.
+        assert (m = {[+ η +]} ⊎ (m ∖ {[+ η +]})) as eq'. multiset_solver.
+        rewrite eq'.
+        exists (q ▷ (m ∖ {[+ η +]})). eapply ParRight.
+        eapply lts_multiset_minus; eauto.
+      + destruct p' as (p' , m').
+        assert (ionly_spec p') as Hyp. eapply ionly_wt; eauto.
+        destruct Hyp as (only_receive & Hyp').
+        eapply lts_refuses_spec1 in mem as ((p'' , m'') & Tr'').
+        inversion Tr''; subst.
+        ++ assert (exist_co_nba μ) as (η & nb & duo). eapply only_receive; eauto.
+           eapply lts_refuses_spec2. exists (q ▷ ({[+ η +]} ⊎ m)).
+           eapply ParRight. simpl in *. eapply lts_multiset_add; eauto.
+        ++ eapply blocking_action_in_ms in not_nb as (eq' & duo' & nb') ; eauto ;subst.
+           eapply lts_refuses_spec2. exists (q ▷ {[+ co μ +]} ⊎ m).
+           eapply ParRight. eapply lts_multiset_add; eauto.
+    - exfalso. eapply (@lts_refuses_spec2 (Q * mb A)). eauto. now eapply nil_refuses.
+    - inversion hcnv; inversion l; subst.
+      + exfalso. eapply (@lts_refuses_spec2 Q); eauto.
+      + destruct (decide (non_blocking μ)) as [nb | not_nb].
+        ++ assert (non_blocking μ). eauto.
+           eapply non_blocking_action_in_ms in nb; eauto ; subst.
+           edestruct (IHhw b2 p) as (t' & hw' & hst' & hsub'); eauto with mdb.
+           eapply H8, wt_act. eapply ParRight.
+           eapply lts_multiset_minus; eauto. eapply wt_nil.
+           exists t'. split. eapply wt_act; eauto. eapply ParRight.
+           eapply lts_multiset_minus;eauto. now split.
+        ++ eapply blocking_action_in_ms in not_nb as (eq & duo & nb); eauto ; subst.
+           edestruct (IHhw ({[+ co μ +]} ⊎ m) p) as (t' & hw' & hst' & hsub'); eauto.
+           eapply H8, wt_act. eapply ParRight. eauto. eapply wt_nil.
+           exists t'. split. eapply wt_act; eauto. eapply ParRight. eauto. now split.
+  Qed.
+
+  Lemma input_only_leq_nil {P Q A : Type} `{
+    @gLtsObaFB P A H gLtsP gLtsEqP V, !FiniteImagegLts P A,
+    @gLtsObaFB Q A H gLtsQ gLtsEqQ W, !FiniteImagegLts Q A,
+    @gLtsObaFB E A H gLtsE gLtsEqE X, !FiniteImagegLts E A, !Testing_Predicate E A attaboy, (∀ e : E, Decision (attaboy e))}
+
+    `{@Prop_of_Inter P E A parallel_inter H gLtsP gLtsE}
+    `{@Prop_of_Inter Q E A parallel_inter H gLtsQ gLtsE}
+
+    `{@Prop_of_Inter P (mb A) A fw_inter H gLtsP MbgLts}
+    `{@Prop_of_Inter (P * mb A) E A parallel_inter H (inter_lts fw_inter) gLtsE}
+
+    `{@Prop_of_Inter Q (mb A) A fw_inter H gLtsQ MbgLts}
+    `{@Prop_of_Inter (Q * mb A) E A parallel_inter H (inter_lts fw_inter) gLtsE}
+
+    `{@gen_spec_conv  _ _ _ _ _ attaboy _ co_of gen_conv, 
+    @gen_spec_acc (P * mb A) (Q * mb A) _ _ _ _ _ attaboy _ co_of gen_acc _ _}
+
+    (p : P) (pr : ionly_spec p) (q : Q) (h : forall α, q ↛{α}) : 
+    @pre_extensional _ _ _ _ _ attaboy _ p q.
+  Proof.
+    now eapply equivalence_bhv_acc_ctx; split; intros ? ?; [eapply nil_cnv | eapply ionly_nil_leq2].
+  Qed. *)
+
+End application.
