theories/Testing_Pre_orders/Must/MustE.v
@@ -1,0 +1,162 @@
+(*
+   Copyright (c) 2024 Nomadic Labs
+   Copyright (c) 2024 Paul Laforgue <paul.laforgue@nomadic-labs.com>
+   Copyright (c) 2024 Léo Stefanesco <leo.stefanesco@mpi-sws.org>
+   Copyright (c) 2025 Gaëtan Lopez <glopez@irif.fr>
+
+   Permission is hereby granted, free of charge, to any person obtaining a copy
+   of this software and associated documentation files (the "Software"), to deal
+   in the Software without restriction, including without limitation the rights
+   to use, copy, modify, merge, publish, distribute, sublicense, and/or sell
+   copies of the Software, and to permit persons to whom the Software is
+   furnished to do so, subject to the following conditions:
+
+   The above copyright notice and this permission notice shall be included in all
+   copies or substantial portions of the Software.
+
+   THE SOFTWARE IS PROVIDED "AS IS", WITHOUT WARRANTY OF ANY KIND, EXPRESS OR
+   IMPLIED, INCLUDING BUT NOT LIMITED TO THE WARRANTIES OF MERCHANTABILITY,
+   FITNESS FOR A PARTICULAR PURPOSE AND NONINFRINGEMENT. IN NO EVENT SHALL THE
+   AUTHORS OR COPYRIGHT HOLDERS BE LIABLE FOR ANY CLAIM, DAMAGES OR OTHER
+   LIABILITY, WHETHER IN AN ACTION OF CONTRACT, TORT OR OTHERWISE, ARISING FROM,
+   OUT OF OR IN CONNECTION WITH THE SOFTWARE OR THE USE OR OTHER DEALINGS IN THE
+   SOFTWARE.
+*)
+
+From stdpp Require Import base decidable gmap finite.
+From Coq Require Import ssreflect.
+From Coq.Program Require Import Equality.
+From Must Require Import gLts Bisimulation Lts_OBA Lts_FW Lts_OBA_FB StateTransitionSystems Termination
+    Must Bar CompletenessAS SoundnessAS Lift Subset_Act FiniteImageLTS WeakTransitions Convergence
+    InteractionBetweenLts MultisetLTSConstruction ForwarderConstruction  ParallelLTSConstruction ActTau
+    Testing_Predicate DefinitionAS Must.
+
+Section preorder.
+
+  (** Extensional definition of Must *)
+
+  Definition must_extensional {P : Type}
+    `{Sts (P * E), attaboy : E -> Prop} 
+    (p : P) (e : E) : Prop :=
+    forall η : max_exec_from (p, e), exists n fex, mex_take_from n η = Some fex 
+          /\ attaboy (fex_from_last fex).2 .
+
+  Definition attaboy_client {P : Type} `{Sts (P * E), attaboy : E -> Prop} (s : (P * E)) := attaboy s.2.
+
+  #[global] Program Instance must_bar {P : Type} {E : Type} `{Sts (P * E)} (attaboy : E -> Prop)
+    `{attaboy_decidable : forall e, Decision (attaboy e)}: Bar (P * E) :=
+    {| bar_pred '(p, e) := attaboy e |}.
+  Next Obligation. intros. destruct x as (p, e). simpl. eauto. Defined.
+
+  Lemma must_intensional_coincide {P : Type}
+    `{Sts (P * E), attaboy : E -> Prop, attaboy_decidable : 
+    forall (e : E), Decision (attaboy e)}
+    (p : P) (e : E) : @intensional_pred (P * E) _ (must_bar attaboy) (p, e) ↔ 
+    @must_sts P E _ attaboy p e.
+  Proof.
+    split.
+    - intros H1. dependent induction H1; subst.
+      + rewrite /bar_pred /= in H1. now eapply m_sts_now.
+      + destruct (attaboy_decidable e).
+        rewrite /bar_pred /= in H1.
+        now eapply m_sts_now. eapply m_sts_step; eauto.
+    - intros hm; dependent induction hm.
+      + constructor 1. 
+        rewrite /bar_pred //=.
+      + constructor 2.
+        * eassumption.
+        * intros (q, e') Hstep. apply H0 =>//=.
+  Qed.
+
+  Lemma must_ext_pred_iff_must_extensional {P : Type}
+    `{StsPE : Sts (P * E), attaboy : E -> Prop, attaboy_decidable : forall (e : E), Decision (attaboy e)}
+    (p : P) (e : E) : @extensional_pred _ _ (must_bar attaboy) (p, e) <-> 
+    @must_extensional P E _ attaboy p e.
+  Proof. split; intros Hme η; destruct (Hme η) as (?&?&?&?).
+         exists x, x0. split. eassumption. simpl. destruct (fex_from_last x0). naive_solver.
+         exists x, x0. split. eassumption. simpl. destruct (fex_from_last x0). naive_solver.
+  Qed.
+
+  Definition pre_extensional
+    {P : Type} {Q : Type} 
+    `{Sts (P * E), Sts (Q * E), attaboy : E -> Prop, attaboy_decidable : forall (e : E), 
+    Decision (attaboy e)}
+    (p : P) (q : Q) : Prop :=
+    forall (e : E), @must_extensional P E _ attaboy p e -> @must_extensional Q E _ attaboy q e.
+
+  (* ************************************************** *)
+
+  Lemma must_extensional_iff_must_sts
+    {P : Type}
+    `{attaboy : E -> Prop, attaboy_decidable : forall (e : E), Decision (attaboy e)}
+    `{gLtsP : @gLts P A H, !FiniteImagegLts P A,
+    gLtsE : !gLts E A, !gLtsEq E A, !Testing_Predicate E A attaboy,  !FiniteImagegLts E A}
+    `{@Prop_of_Inter P E A parallel_inter H gLtsP gLtsE} (* à rajouter en context ? *)
+    (p : P) (e : E) : 
+    @must_extensional P E _ attaboy p e <-> @must_sts P E _ attaboy p e.
+  Proof.
+    split.
+    - intros hm. destruct Testing_Predicate0.
+      eapply must_ext_pred_iff_must_extensional in hm.
+      now eapply must_intensional_coincide, extensional_implies_intensional.
+    - intros hm. destruct Testing_Predicate0.
+      eapply must_intensional_coincide in hm.
+      rewrite <- must_ext_pred_iff_must_extensional.
+      eapply intensional_implies_extensional. eapply hm.
+  Qed.
+
+  Notation "p ⊑ₑ q" := (pre_extensional p q) (at level 70).
+
+  Context `{attaboy : E -> Prop}.
+  Context `{attaboy_dec : forall e, Decision (attaboy e)}.
+  Context `{P : Type}.
+  Context `{Q : Type}.
+  Context `{H : !ExtAction A}.
+  Context `{gLtsP : !gLts P A, !FiniteImagegLts P A}.
+  Context `{gLtsQ : !gLts Q A, !FiniteImagegLts Q A}.
+  Context `{gLtsE : !gLts E A, !FiniteImagegLts E A, gLtsEqE: !gLtsEq E A, !Testing_Predicate E A attaboy}.
+  Context `{@Prop_of_Inter P E A parallel_inter H gLtsP gLtsE}.
+  Context `{@Prop_of_Inter Q E A parallel_inter H gLtsQ gLtsE}.
+
+  (* ************************************************** *)
+
+  Lemma pre_extensional_eq (p : P) (q : Q) : 
+    @pre_extensional P Q _ _ _ attaboy _ p q <-> p ⊑ q.
+    unfold pre_extensional, ctx_pre.
+  Proof.
+    split; intros hpre e.
+    - rewrite <- 2 must_sts_iff_must, <- 2 must_extensional_iff_must_sts; eauto.
+    - rewrite -> 2 must_extensional_iff_must_sts, -> 2 must_sts_iff_must; eauto.
+  Qed.
+
+  Context `{@gLtsObaFB P A H gLtsP gLtsEqP gLtsObaP}.
+  Context `{@gLtsObaFB Q A H gLtsQ gLtsEqQ gLtsObaQ}.
+  Context `{@gLtsObaFB E A H gLtsE gLtsEqE gLtsObaE}.
+
+  Context `{@Prop_of_Inter P (mb A) A fw_inter H gLtsP MbgLts}.
+  Context `{@Prop_of_Inter (P * mb A) E A parallel_inter H (inter_lts fw_inter) gLtsE}.
+  Context `{@Prop_of_Inter Q (mb A) A fw_inter H gLtsQ MbgLts}.
+  Context `{@Prop_of_Inter (Q * mb A) E A parallel_inter H (inter_lts fw_inter) gLtsE}.
+
+  Context `{@PreExtAction A H (P * mb A) FinA PreA PreA_eq PreA_countable 𝝳 Φ (FW_gLts gLtsP)}.
+  Context `{@PreExtAction A H (Q * mb A) FinA PreA PreA_eq PreA_countable 𝝳 Φ (FW_gLts gLtsQ)}.
+  Context `{@AbsAction A H E FinA gLtsE Φ}.
+
+  Context `{igen_conv : @gen_spec_conv E _ _ _ _ attaboy Testing_Predicate0 co_of gen_conv}.
+  Context `{igen_acc : @gen_spec_acc PreA _ _ E _ _ _ _ attaboy Testing_Predicate0 co_of gen_acc (fun x => 𝝳 (Φ x))}.
+
+  (* ************************************************** *)
+
+  (** Equivalence between the extensional definition of the contextual preorder and
+      the alternative, inductive characterisation. *)
+  Theorem equivalence_bhv_acc_ctx (p : P) (q : Q) :
+    @pre_extensional P Q _ _ _ attaboy _ p q <-> (p, ∅) ≼ (q, ∅).
+  Proof.
+    split.
+    - intros hpre%pre_extensional_eq.
+      now eapply lift_fw_ctx_pre, completeness_fw in hpre.
+    - intros hpre%soundness_fw.
+      now eapply pre_extensional_eq, lift_fw_ctx_pre.
+  Qed.
+
+End preorder.
